Checkpoint ctr.Get() proof to fix Goose translation

src/program_proof/fencing/ctr_proof.v
@@ -6,6 +6,7 @@ From Perennial.program_proof Require Export marshal_proof.
 From iris.algebra Require Import cmra.
 From iris.base_logic Require Export mono_nat.
 From Perennial.goose_lang Require Import proph.
+From Perennial.goose_lang Require Import prelude ffi.grove_exit_axiom.
 
 From Perennial.program_proof.fencing Require Export map.
 
@@ -19,6 +20,7 @@ Record ctr_names :=
   epoch_gn : gname ;
   epoch_token_gn : gname ;
   val_gn : gname ;
+  urpc_gn : server_chan_gnames ;
 }.
 
 Implicit Type γ : ctr_names.
@@ -101,9 +103,12 @@ Definition GetPre γ pv e Φ : iProp Σ :=
    else
      True).
 
-Program Definition GetSpec γ :=
+Definition has_GetReply_encoding (l:list u8) (err v:u64) :=
+  has_encoding l [EncUInt64 err; EncUInt64 v].
+
+Program Definition Get_spec γ :=
   λ (reqData:list u8), λne (Φ : list u8 -d> iPropO Σ),
-  (∃ (pv:proph_id) (repV:u64) e,
+  (∃ (pv pe:proph_id) (repV:u64) e,
   proph_once pv repV ∗
   ⌜has_encoding reqData [EncUInt64 e]⌝ ∗
   (|={⊤,∅}=> ∃ latestEpoch, if decide (int.Z latestEpoch < int.Z e)%Z then
@@ -112,16 +117,180 @@ Program Definition GetSpec γ :=
                             (∀ v, own_val γ e v (1/2)%Qp ∗
                                            own_val γ latestEpoch v (1/2)%Qp ∗
                                            own_latest_epoch γ e (1/2)%Qp
-                                  ={∅,⊤}=∗ (∀ l, ⌜has_encoding l [EncUInt64 v]⌝ -∗ proph_once pv v -∗ Φ l))
+                                  ={∅,⊤}=∗ (∀ l, ⌜has_GetReply_encoding l 0 v⌝ -∗ proph_once pv v -∗ Φ l))
    else if decide (int.Z latestEpoch = int.Z e) then
     ∃ v, own_latest_epoch γ latestEpoch (1/2)%Qp ∗
      own_val γ e v (1/2)%Qp ∗
-    (own_val γ e v (1/2)%Qp ∗ own_latest_epoch γ e (1/2)%Qp ={∅,⊤}=∗ (∀ l, ⌜has_encoding l [EncUInt64 v]⌝ -∗ proph_once pv v -∗ Φ l))
+    (own_val γ e v (1/2)%Qp ∗ own_latest_epoch γ e (1/2)%Qp ={∅,⊤}=∗ (∀ l, ⌜has_GetReply_encoding l 0 v⌝ -∗ proph_once pv v -∗ Φ l))
    else
-     True))%I.
+     (* FIXME: in this case, the server returns *)
+      (∀ l, ⌜has_GetReply_encoding l 1 0⌝ -∗ proph_once pe true -∗ Φ l)
+     ))%I.
 Next Obligation.
   solve_proper.
 Defined.
+
+Context `{!rpcregG Σ}.
+
+Definition is_host (host:u64) γ : iProp Σ :=
+  handler_spec γ.(urpc_gn) host (U64 0) (Get_spec γ) ∗
+  handlers_dom γ.(urpc_gn) {[ (U64 0) ]}
+.
+
+Definition own_Clerk γ (ck:loc) : iProp Σ :=
+  ∃ (cl:loc) host,
+  "#Hcl" ∷ readonly (ck ↦[Clerk :: "cl"] #cl) ∗
+  "#Hcl_own" ∷ is_RPCClient cl host ∗
+  "#Hhost" ∷ is_host host γ
+.
+
+Lemma wp_Clerk__Get γ ck (e:u64) :
+  ∀ Φ,
+  own_Clerk γ ck -∗
+  (|={⊤,∅}=> ∃ latestEpoch, if decide (int.Z latestEpoch < int.Z e)%Z then
+      own_latest_epoch γ latestEpoch (1/2)%Qp ∗
+      own_unused_epoch γ e ∗
+                            (∀ v, own_val γ e v (1/2)%Qp ∗
+                                           own_val γ latestEpoch v (1/2)%Qp ∗
+                                           own_latest_epoch γ e (1/2)%Qp
+                                           ={∅,⊤}=∗ (own_Clerk γ ck -∗ Φ #v))
+   else if decide (int.Z latestEpoch = int.Z e) then
+    ∃ v, own_latest_epoch γ latestEpoch (1/2)%Qp ∗
+     own_val γ e v (1/2)%Qp ∗
+    (own_val γ e v (1/2)%Qp ∗ own_latest_epoch γ e (1/2)%Qp ={∅,⊤}=∗ (own_Clerk γ ck -∗ Φ #v))
+   else
+     True) -∗
+    WP Clerk__Get #ck #e {{ Φ }}.
+Proof.
+  iIntros (Φ) "Hck Hupd".
+  wp_lam.
+  wp_pures.
+  wp_apply (wp_new_enc).
+  iIntros (enc) "Henc".
+  wp_pures.
+  wp_apply (wp_Enc__PutInt with "Henc").
+  { done. }
+  iIntros "Henc".
+  wp_pures.
+  wp_apply (wp_Enc__Finish with "Henc").
+  iIntros (req_sl reqData) "(%Hreq_enc & %Hreq_len & Hreq_sl)".
+  wp_pures.
+  wp_apply (wp_NewProph_once (T:=u64)).
+  iIntros (valProph v) "Hprophv".
+  wp_apply (wp_NewProph_once (T:=bool)).
+  iIntros (errProph err) "Hprophe".
+  wp_pures.
+
+  wp_apply (wp_ref_of_zero).
+  { done. }
+  iIntros (rep) "Hrep".
+  wp_pures.
+  iNamed "Hck".
+  wp_loadField.
+  wp_apply (wp_Client__Call _ _ _ _ _ _ _ _ _ _
+                          (λ (l:list u8), ∃ v e, ⌜has_GetReply_encoding l e v⌝ ∗
+                                  if (decide (int.Z e = 0)) then
+                                    (own_Clerk γ ck -∗ Φ #v) ∗ proph_once valProph v
+                                  else
+                                    proph_once errProph true)%I
+             with "[$Hreq_sl $Hrep $Hcl_own Hupd Hprophv Hprophe]").
+  {
+    iDestruct "Hhost" as "[$ _]".
+    iAssert (□ proph_once valProph v)%I with "[Hprophv]" as "Hprophv".
+    { admit. } (* FIXME: this is false; we're gonna need another piece of ghost state that matches the value of the prophecy, but is persistent *)
+    iAssert (□ proph_once errProph e)%I with "[Hprophe]" as "Hprophe".
+    { admit. }
+    iDestruct "Hprophv" as "#Hprophv".
+    iDestruct "Hprophe" as "#Hprophe".
+    do 2 iModIntro.
+    iAssert
+      (|={⊤,∅}=> ∃ latestEpoch, if decide (int.Z latestEpoch < int.Z e)%Z then
+      own_latest_epoch γ latestEpoch (1/2)%Qp ∗
+      own_unused_epoch γ e ∗
+                            (∀ v, own_val γ e v (1/2)%Qp ∗
+                                           own_val γ latestEpoch v (1/2)%Qp ∗
+                                           own_latest_epoch γ e (1/2)%Qp
+                                           ={∅,⊤}=∗ (own_Clerk γ ck -∗ Φ #v))
+   else if decide (int.Z latestEpoch = int.Z e) then
+    ∃ v, own_latest_epoch γ latestEpoch (1/2)%Qp ∗
+     own_val γ e v (1/2)%Qp ∗
+    (own_val γ e v (1/2)%Qp ∗ own_latest_epoch γ e (1/2)%Qp ={∅,⊤}=∗ (own_Clerk γ ck -∗ Φ #v))
+   else
+     True)%I with "[]" as "Hupd".
+    { admit. } (* FIXME: will need to put this or the reply in escrow *)
+    simpl.
+    iExists valProph,errProph,_,_; iFrame "Hprophv".
+    iSplitL ""; first done.
+    iMod "Hupd".
+    iModIntro.
+    iDestruct "Hupd" as (latestEpoch) "Hupd".
+    iExists latestEpoch.
+    destruct (decide (int.Z latestEpoch < int.Z e)%Z).
+    {
+      iDestruct "Hupd" as "($ & $ & Hupd)".
+      iIntros (val) "Hpre".
+      iDestruct ("Hupd" with "Hpre") as "Hupd".
+      iMod "Hupd".
+      iModIntro.
+      iIntros.
+      iExists _,_.
+      iSplitL ""; first done.
+      setoid_rewrite decide_True; last done.
+      iFrame "Hupd".
+      iFrame.
+    }
+    { (* similar to above *)
+      admit.
+    }
+  }
+
+  iIntros (errCode) "(_ & Hreq_sl & Hpost)".
+  (* will be able to show that errCode = None iff err = false by prophecy.Resolve *)
+
+  wp_pures.
+  destruct errCode.
+  { (* case: error *)
+    rewrite bool_decide_false; last first.
+    { by destruct c. }
+    wp_pures.
+    wp_apply (wp_Exit).
+    by iIntros.
+  (* FIXME: I don't know if I need to prophesize about the error code; if
+     there's an error, we just exit, and the caller finds out nothing *)
+  }
+  (* case: no error *)
+  wp_pures.
+  iNamed "Hpost".
+  iDestruct "Hpost" as "(Hrep & Hrep_sl & Hpost)".
+  wp_load.
+  clear v.
+  clear err.
+  iDestruct "Hpost" as (v err) "(%Hrep_enc & Hpost)".
+
+  (* TODO: move this to a different lemma *)
+  wp_lam.
+  iDestruct (is_slice_to_small with "Hrep_sl") as "Hrep_small".
+  wp_apply (wp_new_dec with "[$Hrep_small]").
+  { done. }
+  iIntros (dec) "Hdec".
+  wp_pures.
+  wp_apply (wp_allocStruct).
+  { naive_solver. }
+  iIntros (r) "Hr".
+  iDestruct (struct_fields_split with "Hr") as "HH".
+  iNamed "HH".
+  simpl.
+  wp_pures.
+  wp_apply (wp_Dec__GetInt with "Hdec").
+  iIntros "Hdec".
+  wp_storeField.
+
+  wp_apply (wp_Dec__GetInt with "Hdec").
+  iIntros "Hdec".
+  wp_storeField.
+  wp_pures.
+  (* TODO: move the above to a different lemma *)
+Admitted.
 
 Lemma wp_Server__Get γ s (e:u64) (rep:loc) (dummy_err dummy_val:u64) :
   is_Server γ s -∗
@@ -157,29 +326,7 @@ Proof.
 Admitted.
 
 
-Definition own_Clerk γ (ck:loc) : iProp Σ.
-Admitted.
-
 (* NOTE: consider lt_eq_lt_dec: ∀ n m : nat, {n < m} + {n = m} + {m < n} *)
-Lemma wp_Clerk__Get γ ck (e:u64) :
-  ∀ Φ,
-  own_Clerk γ ck -∗
-  (|={⊤,∅}=> ∃ latestEpoch, if decide (int.Z latestEpoch < int.Z e)%Z then
-      own_latest_epoch γ latestEpoch (1/2)%Qp ∗
-      own_unused_epoch γ e ∗
-                            (∀ v, own_val γ e v (1/2)%Qp ∗
-                                           own_val γ latestEpoch v (1/2)%Qp ∗
-                                           own_latest_epoch γ e (1/2)%Qp
-                                           ={∅,⊤}=∗ (own_Clerk γ ck -∗ Φ #v))
-   else if decide (int.Z latestEpoch = int.Z e) then
-    ∃ v, own_latest_epoch γ latestEpoch (1/2)%Qp ∗
-     own_val γ e v (1/2)%Qp ∗
-    (own_val γ e v (1/2)%Qp ∗ own_latest_epoch γ e (1/2)%Qp ={∅,⊤}=∗ (own_Clerk γ ck -∗ Φ #v))
-   else
-     True) -∗
-    WP Clerk__Get #ck #e {{ Φ }}.
-Proof.
-Admitted.
 
 Lemma wp_Clerk__Put γ ck (e v:u64) :
   ∀ Φ,
